Dadas las siguientes funciones l√≥gicas:


1.

$${\color{red}\overline{Z = A + B.\overline{C} \oplus \overline{B}}}$$

```math
2. Z = \overline{A \cdot \overline{(B + \overline{C}}}
```

```math
3. Z = A \cdot B \cdot C
```

```math
4. Z = A \oplus B \cdot C + A \cdot C
```

```math
5. Z = A \oplus B \cdot C + A + B + D
```

```math
6. Z = A + B \oplus C
```

```math
7. Z = (A + B \cdot C) + (B + C)
```

```math
8. Z = ((A + B) \cdot C) + (A + D \cdot C)
```

```math
9. Z = (A \oplus C) \cdot (A + B) \cdot (C + D)
```

```math
10. Z = (A + B + C) \oplus C
```

```math
11. Z = (A \cdot B) + (C \oplus D)
```

```math
12. Z = (A + B \cdot C) \cdot (B + C \cdot D)
```

```math
13. Z = (A + B \cdot C) \cdot (A + B)
```

```math
14. Z = A + B + C + D
```

```math
15. Z = (A + B) \oplus (B \cdot C) + D
```

```math
16. Z = (A + B \oplus C) + D
```

```math
17. Z = A + B \cdot (C + D)
```

```math
18. Z = A \oplus B \cdot C + D
```

```math
19. Z = A \cdot B \cdot C + D
```

```math
20. Z = \bar{A + B + C} + D
```


21. $ Z = (A \oplus B) \oplus C $

```math
22. Z = (A + C) \oplus (B \cdot D)
```

```math
23. Z = A \oplus B \cdot C + A \cdot B + D
```

```math
24. Z = (A + B) \cdot (C + D)
```

```math
25. Z = A \oplus B + C \cdot (A + D)
```

```math
26. Z = (A + B) \cdot (C + B)
```
